theories/iris/logrel/module.v
@@ -1,47 +1,19 @@
-Require Import RichWasm.compiler.prelude.
-From RichWasm.iris Require Import memory util.
-Require Import RichWasm.iris.logrel.instr.
-Require Import RichWasm.iris.host.iris_host.
-Require Import RichWasm.syntax.
+Require Import RichWasm.typing.
+Require Import RichWasm.compiler.module.
+Require Import RichWasm.iris.rules.iris_rules.
+Require Import RichWasm.iris.logrel.
 
-Section Relations.
+Set Bullet Behavior "Strict Subproofs".
+Set Default Goal Selector "!".
 
-  Context `{!logrel_na_invs Σ}.
-  Context `{!wasmG Σ}.
-  Context `{!richwasmG Σ}.
-  Context `{!wasmG Σ}.
-  Context `{!hvisG Σ}.
-  Context `{!hmsG Σ}.
-  Context `{!hasG Σ}.
+Section Fundamental.
 
-  Variable rti : rt_invariant Σ.
-  Variable sr : store_runtime.
+  Context `{Σ : gFunctors}.
 
-  (* TODO *)
-  Definition module_interp (ω : module_type) (mr : module_runtime) (m : W.module) : iProp Σ :=
-    (∀ i imports exports,
-       i ↪[mods] m -∗
-       (* TODO: Assert that indices in the module point to the global runtime funcaddrs. *)
-       ([∗ list] i ↦ ϕ ∈ ω.(mt_imports),
-          ∃ bs j cl,
-            N.of_nat i ↪[vis] datatypes.Build_module_export bs (MED_func j) ∗
-              N.of_nat (funcimm j) ↦[wf] cl ∗
-              closure_interp rti sr senv_empty ϕ cl ∗
-              ⌜imports !! (funcimm mr.(mr_func_user) + i)%nat = Some (N.of_nat (funcimm j))⌝) -∗
-       ([∗ list] i ↦ '_ ∈ ω.(mt_exports),
-          ∃ bs j,
-            N.of_nat i ↪[vis] datatypes.Build_module_export bs (MED_func j) ∗
-              ⌜exports !! i = Some (N.of_nat (funcimm j))⌝) -∗
-       WP (([ID_instantiate exports i imports], []) : host_expr) @ top
-          {{ v, ⌜v = immHV []⌝ ∗
-                  i ↪[mods] m ∗
-                  ([∗ list] i ↦ ϕ ∈ ω.(mt_exports),
-                     ∃ j cl, (* TODO: same j as precond *)
-                       N.of_nat (funcimm j) ↦[wf] cl ∗
-                         closure_interp rti sr senv_empty ϕ cl) }})%I.
+  Theorem fundamental_module m m' ω :
+    has_module_type m ω ->
+    run_modgen (compile_module m) mod_empty = inr (tt, m') ->
+    ⊢ @has_module_type_sem Σ m' ω.
+  Admitted.
 
-  (* TODO *)
-  Definition has_module_type_sem (m : W.module) (ω : module_type) : iProp Σ :=
-    True%I.
-
-End Relations.
+End Fundamental.
