theories/iris/wp_codegen.v
@@ -4,7 +4,7 @@ From stdpp Require Import list.
 From RichWasm Require Import syntax typing util.
 From RichWasm.compiler Require Import prelude accum codegen.
 From RichWasm.iris Require Import autowp cwp lenient_wp logpred.
-Require Import RichWasm.iris.logrel.instr.
+Require Import RichWasm.iris.logrel.
 
 Module W := RichWasm.wasm.operations.
 
